More monotonicity proofs

theories/Shallow/Executor.v
@@ -28,10 +28,13 @@
 
 From Coq Require Import
      Bool.Bool
+     Classes.Morphisms
      Lists.List
      NArith.NArith
+     Program.Basics
      Program.Tactics
      Strings.String
+     Relations.Relation_Definitions
      ZArith.BinInt.
 From Equations Require Import
      Equations.
@@ -47,6 +50,7 @@ From stdpp Require base list option.
 Import ctx.notations.
 Import env.notations.
 Import ListNotations.
+Import SignatureNotations.
 
 Set Implicit Arguments.
 
@@ -62,7 +66,20 @@ Module Type ShallowExecOn
   Definition CStoreSpec (Γ1 Γ2 : PCtx) (A : Type) : Type :=
     (A -> CStore Γ2 -> SCHeap -> Prop) -> CStore Γ1 -> SCHeap -> Prop.
 
+  Definition MStoreSpec (Γ1 Γ2 : PCtx) [A] (MA : relation A) :
+    relation (CStoreSpec Γ1 Γ2 A) :=
+    (MA ==> CStore Γ2 ::> SCHeap ::> impl) ==> CStore Γ1 ::> SCHeap ::> impl.
+  #[global] Arguments MStoreSpec Γ1 Γ2 [A] MA.
+
+  Definition Exec := forall Γ τ (s : Stm Γ τ), CStoreSpec Γ Γ (Val τ).
+
+  Notation MonotonicExec exec :=
+    (forall Γ τ (s : Stm Γ τ),
+       Monotonic (MStoreSpec Γ Γ eq) (exec Γ τ s)).
+
   Module CStoreSpec.
+
+    Import (hints) CHeapSpec.
 
     Section Basic.
 
@@ -107,6 +124,61 @@ Module Type ShallowExecOn
         fun Δ => lift_purespec (CPureSpec.demonic_ctx Δ).
       #[global] Arguments demonic_ctx {N Γ} Δ.
 
+      Lemma mon_evalStoreSpec' {Γ1 Γ2} `{MA : relation A} :
+        Monotonic (MStoreSpec Γ1 Γ2 MA ==> CStore Γ1 ::> MHeapSpec MA) evalStoreSpec.
+      Proof. intros ? ? rm δ ? ? rΦ. apply rm. intros ? ? ? _. now apply rΦ. Qed.
+
+      #[export] Instance mon_evalStoreSpec {Γ1 Γ2} `{MA : relation A} ma δ1 :
+        Monotonic (MStoreSpec Γ1 Γ2 MA) ma ->
+        Monotonic (MHeapSpec MA) (evalStoreSpec ma δ1).
+      Proof. intros rma. now apply mon_evalStoreSpec'. Qed.
+
+      Lemma mon_lift_purespec' `{MA : relation A} {Γ} :
+        Monotonic (MPureSpec MA ==> MStoreSpec Γ Γ MA) lift_purespec.
+      Proof. intros ? ? rm ? ? rΦ ? ?. apply rm. intros ? ? ?. now apply rΦ. Qed.
+
+      #[export] Instance mon_lift_purespec `{MA : relation A} {Γ} m :
+        Monotonic (MPureSpec MA) m -> Monotonic (MStoreSpec Γ Γ MA) (lift_purespec m).
+      Proof. intros rm. now apply mon_lift_purespec'. Qed.
+
+      Lemma mon_lift_heapspec' `{MA : relation A} {Γ} :
+        Monotonic (MHeapSpec MA ==> MStoreSpec Γ Γ MA) lift_heapspec.
+      Proof. intros ? ? rm ? ? rΦ ?. apply rm. intros ? ? ?. now apply rΦ. Qed.
+
+      #[export] Instance mon_lift_heapspec `{MA : relation A} {Γ} m :
+        Monotonic (MHeapSpec MA) m -> Monotonic (MStoreSpec Γ Γ MA) (lift_heapspec m).
+      Proof. intros rm. now apply mon_lift_heapspec'. Qed.
+
+      Lemma mon_pure' `{MA : relation A} {Γ} :
+        Monotonic (MA ==> MStoreSpec Γ Γ MA) pure.
+      Proof. unfold pure. firstorder. Qed.
+
+      #[export] Instance mon_pure `{MA : relation A} {Γ}  x :
+        Monotonic MA x -> Monotonic (MStoreSpec Γ Γ MA) (pure x).
+      Proof. unfold pure. firstorder. Qed.
+
+      Lemma mon_bind' `{MA : relation A, RB : relation B} {Γ1 Γ2 Γ3} :
+        Monotonic (MStoreSpec Γ1 Γ2 MA ==> (MA ==> MStoreSpec Γ2 Γ3 RB) ==> MStoreSpec Γ1 Γ3 RB) bind.
+      Proof.
+        intros ? ? rm ? ? rf ? ? rΦ. apply rm.
+        intros ? ? ra. apply rf. apply ra. apply rΦ.
+      Qed.
+
+      #[export] Instance mon_bind `{MA : relation A, RB : relation B} {Γ1 Γ2 Γ3}
+        (m : CStoreSpec Γ1 Γ2 A) (f : A -> CStoreSpec Γ2 Γ3 B) :
+        Monotonic (MStoreSpec Γ1 Γ2 MA) m ->
+        Monotonic (MA ==> MStoreSpec Γ2 Γ3 RB) f ->
+        Monotonic (MStoreSpec Γ1 Γ3 RB) (bind m f).
+      Proof. intros rm rf. eapply mon_bind'; eauto. Qed.
+
+      #[export] Instance mon_error `{MA : relation A} {Γ1 Γ2} :
+        Monotonic (MStoreSpec Γ1 Γ2 MA) error.
+      Proof. easy. Qed.
+
+      #[export] Instance mon_block `{MA : relation A} {Γ1 Γ2} :
+        Monotonic (MStoreSpec Γ1 Γ2 MA) block.
+      Proof. easy. Qed.
+
     End Basic.
 
     Module CStoreSpecNotations.
@@ -139,6 +211,26 @@ Module Type ShallowExecOn
         lift_purespec (CPureSpec.assert_eq_env δ δ').
       Definition assert_eq_nenv {N Γ} {Δ : NCtx N Ty} (δ δ' : NamedEnv Val Δ) : CStoreSpec Γ Γ unit :=
         lift_purespec (CPureSpec.assert_eq_nenv δ δ').
+
+      #[export] Instance mon_assume_formula {Γ} (fml : Prop) :
+        Monotonic (MStoreSpec Γ Γ eq) (assume_formula fml).
+      Proof. typeclasses eauto. Qed.
+
+      #[export] Instance mon_assert_formula {Γ} (fml : Prop) :
+        Monotonic (MStoreSpec Γ Γ eq) (assert_formula fml).
+      Proof. typeclasses eauto. Qed.
+
+      #[export] Instance mon_assert_pathcondition {Γ} (fml : Prop) :
+        Monotonic (MStoreSpec Γ Γ eq) (assert_pathcondition fml).
+      Proof. typeclasses eauto. Qed.
+
+      #[export] Instance mon_assert_eq_env {Γ} {Δ : Ctx Ty} (δ δ' : Env Val Δ) :
+        Monotonic (MStoreSpec Γ Γ eq) (assert_eq_env δ δ').
+      Proof. typeclasses eauto. Qed.
+
+      #[export] Instance mon_assert_eq_nenv {N Γ} {Δ : NCtx N Ty} (δ δ' : NamedEnv Val Δ) :
+        Monotonic (MStoreSpec Γ Γ eq) (assert_eq_nenv δ δ').
+      Proof. typeclasses eauto. Qed.
 
     End AssumeAssert.
 
@@ -180,6 +272,38 @@ Module Type ShallowExecOn
         fun POST δ => POST tt (δ ⟪ x ↦ v ⟫).
       Global Arguments assign {Γ} x {σ xIn} v.
 
+      #[export] Instance mon_pushpop `{MA : relation A} {Γ1 Γ2 x σ} (v : Val σ)
+        (d : CStoreSpec (Γ1 ▻ x∷σ) (Γ2 ▻ x∷σ) A) :
+        Monotonic (MStoreSpec (Γ1 ▻ x∷σ) (Γ2 ▻ x∷σ) MA) d ->
+        Monotonic (MStoreSpec Γ1 Γ2 MA) (pushpop v d).
+      Proof. intros md P Q PQ ?. apply md. intros ? ? ma ?. now apply PQ. Qed.
+
+      #[export] Instance mon_pushspops `{MA : relation A} {Γ1 Γ2 Δ} (δΔ : CStore Δ)
+        (d : CStoreSpec (Γ1 ▻▻ Δ) (Γ2 ▻▻ Δ) A) :
+        Monotonic (MStoreSpec (Γ1 ▻▻ Δ) (Γ2 ▻▻ Δ) MA) d ->
+        Monotonic (MStoreSpec Γ1 Γ2 MA) (pushspops δΔ d).
+      Proof. intros md P Q PQ ?. apply md. intros ? ? ma ?. now apply PQ. Qed.
+
+      #[export] Instance mon_get_local {Γ} :
+        Monotonic (MStoreSpec Γ Γ eq) get_local.
+      Proof. intros P Q PQ ?. now apply PQ. Qed.
+
+      #[export] Instance mon_put_local {Γ1 Γ2} (δ : CStore Γ2) :
+        Monotonic (MStoreSpec Γ1 Γ2 eq) (put_local δ).
+      Proof. intros P Q PQ ?. now apply PQ. Qed.
+
+      #[export] Instance mon_eval_exp {Γ σ} (e : Exp Γ σ) :
+        Monotonic (MStoreSpec Γ Γ eq) (eval_exp e).
+      Proof. intros P Q PQ ?. now apply PQ. Qed.
+
+      #[export] Instance mon_eval_exps {Γ} {σs : PCtx} (es : NamedEnv (Exp Γ) σs) :
+        Monotonic (MStoreSpec Γ Γ eq) (eval_exps es).
+      Proof. intros P Q PQ ?. now apply PQ. Qed.
+
+      #[export] Instance mon_assign {Γ} x {σ} {xIn : x∷σ ∈ Γ} (v : Val σ) :
+        Monotonic (MStoreSpec Γ Γ eq) (assign x v).
+      Proof. intros P Q PQ ?. now apply PQ. Qed.
+
     End State.
 
     Section ProduceConsume.
@@ -198,6 +322,30 @@ Module Type ShallowExecOn
         lift_heapspec (CHeapSpec.read_register r).
       Definition write_register {Γ τ} (r : 𝑹𝑬𝑮 τ) (v : Val τ) : CStoreSpec Γ Γ (Val τ) :=
         lift_heapspec (CHeapSpec.write_register r v).
+
+      Lemma mon_produce {Γ Σ} (asn : Assertion Σ) (ι : Valuation Σ) :
+        Monotonic (MStoreSpec Γ Γ eq) (produce asn ι).
+      Proof. typeclasses eauto. Qed.
+
+      Lemma mon_consume {Γ Σ} (asn : Assertion Σ) (ι : Valuation Σ) :
+        Monotonic (MStoreSpec Γ Γ eq) (consume asn ι).
+      Proof. typeclasses eauto. Qed.
+
+      Lemma mon_produce_chunk {Γ} (c : SCChunk) :
+        Monotonic (MStoreSpec Γ Γ eq) (produce_chunk c).
+      Proof. typeclasses eauto. Qed.
+
+      Lemma mon_consume_chunk {Γ} (c : SCChunk) :
+        Monotonic (MStoreSpec Γ Γ eq) (consume_chunk c).
+      Proof. typeclasses eauto. Qed.
+
+      #[export] Instance mon_read_register {Γ τ} (r : 𝑹𝑬𝑮 τ) :
+        Monotonic (MStoreSpec Γ Γ eq) (read_register r).
+      Proof. typeclasses eauto. Qed.
+
+      #[export] Instance mon_write_register {Γ τ} (r : 𝑹𝑬𝑮 τ) (v : Val τ) :
+        Monotonic (MStoreSpec Γ Γ eq) (write_register (Γ := Γ) r v).
+      Proof. apply mon_lift_heapspec, CHeapSpec.mon_write_register. Qed.
 
     End ProduceConsume.
 
@@ -283,6 +431,17 @@ Module Type ShallowExecOn
               exec_aux k
             end.
 
+        Context {mon_rec : MonotonicExec rec}.
+
+        #[export] Instance mon_exec_aux : MonotonicExec exec_aux.
+        Proof.
+          intros Γ τ s. induction s; cbn - [Val]; try typeclasses eauto.
+          destruct CEnv.
+          - typeclasses eauto.
+          - intros P Q PQ ? ?. apply mon_rec.
+            intros ? ? ? ?. now apply PQ.
+        Qed.
+
       End ExecAux.
       Arguments exec_aux rec {Γ τ} !s.
 
@@ -292,9 +451,12 @@ Module Type ShallowExecOn
         | O   => fun _ _ _ => error
         | S n => @exec_aux (@exec n)
         end.
-      Global Arguments exec _ {_ _} s _ _ _ : simpl never.
+
+      #[export] Instance mon_exec fuel : MonotonicExec (exec fuel).
+      Proof. induction fuel; cbn; typeclasses eauto. Qed.
 
     End Exec.
+    #[global] Arguments exec _ {_ _} s : simpl never.
 
     Section WithFuel.
 
@@ -313,6 +475,10 @@ Module Type ShallowExecOn
 
       Definition vcgen {Δ τ} (c : SepContract Δ τ) (body : Stm Δ τ) : Prop :=
         CHeapSpec.run (exec_contract c body).
+
+      Lemma mon_exec_contract {Δ τ} (c : SepContract Δ τ) (s : Stm Δ τ) :
+        Monotonic (MHeapSpec eq) (exec_contract c s).
+      Proof. destruct c. typeclasses eauto. Qed.
 
     End WithFuel.
 
