theories/Shallow/Soundness.v
@@ -54,133 +54,6 @@ Module Type Soundness
   Import CStoreSpec.
   Import ProgramLogic.
 
-  (* This section verifies the monotonicity of the calculated predicate
-     transformers. Which is a necessity for the main soundness theorems. *)
-  Section Monotonicity.
-
-    Definition Monotonic {Γ1 Γ2 A} (m : CStoreSpec Γ1 Γ2 A) : Prop :=
-      forall
-        (P Q : A -> CStore Γ2 -> SCHeap -> Prop)
-        (PQ : forall x δ h, P x δ h -> Q x δ h),
-      forall δ h, m P δ h -> m Q δ h.
-
-    (* Stronger version for those that do not change the store. *)
-    Definition Monotonic' {Γ A} (m : CStoreSpec Γ Γ A) : Prop :=
-      forall δ
-        (P Q : A -> CStore Γ -> SCHeap -> Prop)
-        (PQ : forall x h, P x δ h -> Q x δ h),
-      forall h, m P δ h -> m Q δ h.
-
-    Lemma consume_chunk_monotonic {Γ} (c : SCChunk) :
-      Monotonic' (consume_chunk (Γ := Γ) c).
-    Proof.
-      unfold consume_chunk, Monotonic. intros δ P Q PQ.
-      apply CHeapSpec.mon_consume_chunk. intros ? ? ->.
-      unfold pointwise_relation, impl. apply PQ.
-    Qed.
-
-    Lemma produce_chunk_monotonic {Γ} (c : SCChunk) :
-      Monotonic' (produce_chunk (Γ := Γ) c).
-    Proof.
-      unfold produce_chunk, Monotonic. intros δ P Q PQ.
-      apply CHeapSpec.mon_produce_chunk. intros ? ? ->.
-      unfold pointwise_relation, impl. apply PQ.
-    Qed.
-
-    Lemma consume_monotonic {Γ Σ} {ι : Valuation Σ} {asn : Assertion Σ} :
-      Monotonic' (consume (Γ := Γ) asn ι).
-    Proof.
-      unfold consume, Monotonic'. intros * PQ δ.
-      apply CHeapSpec.mon_consume. intros ? ? ->.
-      unfold pointwise_relation, impl. apply PQ.
-    Qed.
-
-    Lemma produce_monotonic {Γ Σ} {ι : Valuation Σ} {asn : Assertion Σ} :
-      Monotonic' (produce (Γ := Γ) asn ι).
-    Proof.
-      unfold produce, Monotonic'. intros * PQ.
-      apply CHeapSpec.mon_produce. intros ? ? ->.
-      unfold pointwise_relation, impl. apply PQ.
-    Qed.
-
-    Lemma read_register_monotonic {Γ τ} (r : 𝑹𝑬𝑮 τ) :
-      Monotonic (read_register (Γ := Γ) r).
-    Proof.
-      unfold read_register, Monotonic. intros * PQ δ.
-      apply CHeapSpec.mon_read_register. intros ? ? ->.
-      unfold pointwise_relation, impl. apply PQ.
-    Qed.
-
-    Lemma write_register_monotonic {Γ τ} (r : 𝑹𝑬𝑮 τ) (v : Val τ) :
-      Monotonic (write_register (Γ := Γ) r v).
-    Proof.
-      unfold write_register, Monotonic. intros * PQ δ.
-      apply CHeapSpec.mon_write_register. intros ? ? ->.
-      unfold pointwise_relation, impl. apply PQ.
-    Qed.
-
-    Lemma call_lemma_monotonic {Γ Δ} (lem : Lemma Δ) (δΔ : CStore Δ) :
-      Monotonic (call_lemma (Γ := Γ) lem δΔ).
-    Proof.
-      unfold call_lemma, Monotonic. intros * PQ δ.
-      apply CHeapSpec.mon_call_lemma. intros ? ? ->.
-      unfold pointwise_relation, impl. apply PQ.
-    Qed.
-
-    Lemma call_contract_monotonic {Γ Δ τ} (c : SepContract Δ τ) (δΔ : CStore Δ) :
-      Monotonic (call_contract (Γ := Γ) c δΔ).
-    Proof.
-      unfold call_contract, Monotonic. intros * PQ δ.
-      apply CHeapSpec.mon_call_contract. intros ? ? ->.
-      unfold pointwise_relation, impl. apply PQ.
-    Qed.
-
-    Definition MonotonicExec (ex : Exec) : Prop :=
-      forall Γ τ (s : Stm Γ τ),
-      Monotonic (ex _ _ s).
-
-    Lemma exec_aux_monotonic rec (rec_mono : MonotonicExec rec) :
-      MonotonicExec (@exec_aux rec).
-    Proof.
-      unfold MonotonicExec. intros ? ? s.
-      induction s; cbn; intros P Q PQ *;
-        cbv [pure bind angelic pushpop pushspops
-               put_local get_local eval_exp eval_exps assign].
-      - auto.
-      - auto.
-      - apply IHs1. intros *. apply IHs2. auto.
-      - apply IHs. auto.
-      - apply IHs. auto.
-      - destruct (CEnv f); cbn; auto.
-        + apply call_contract_monotonic; auto.
-        + apply rec_mono; auto.
-      - apply IHs. auto.
-      - apply call_contract_monotonic; auto.
-      - apply call_lemma_monotonic; intros ? ? ?.
-        apply IHs. auto.
-      - apply IHs1. intros ? ? ?. apply IHs2. auto.
-      - intros HYP Heq. specialize (HYP Heq). revert HYP.
-        apply IHs; auto.
-      - auto.
-      - apply IHs. intros ? ? ?.
-        rewrite !wp_demonic_pattern_match.
-        destruct pattern_match_val.
-        apply H; auto.
-      - now apply read_register_monotonic.
-      - now apply write_register_monotonic.
-      - apply IHs; intros *; apply H; auto.
-      - apply IHs; auto.
-    Qed.
-
-    Lemma exec_monotonic n : MonotonicExec (@exec n).
-    Proof.
-      induction n; cbn.
-      - unfold MonotonicExec, Monotonic; cbn; auto.
-      - now apply exec_aux_monotonic.
-    Qed.
-
-  End Monotonicity.
-
   Section Soundness.
 
     Import iris.proofmode.tactics.
@@ -194,80 +67,26 @@ Module Type Soundness
     Definition liftP {Γ} (POST : CStore Γ -> L) : CStore Γ -> SCHeap -> Prop :=
       fun δ h => interpret_scheap h ⊢ POST δ.
 
-    Lemma consume_chunk_sound {Γ} (c : SCChunk) (POST : CStore Γ -> L) :
-      forall δ h,
-        consume_chunk c (fun _ => liftP POST) δ h ->
-        interpret_scheap h ⊢ interpret_scchunk c ∗ POST δ.
-    Proof.
-      unfold consume_chunk. intros δ h ->%CPureSpec.wp_consume_chunk.
-      apply bi.sep_mono'. easy.
-      apply bi.exist_elim. intros h'.
-      now apply bi.pure_elim_r.
-    Qed.
-
-    Lemma assert_formula_sound {Γ Σ} {ι : Valuation Σ} {fml : Formula Σ}
-      (POST : CStore Γ -> L) :
-      forall δ h,
-        assert_formula (instprop fml ι)
-          (fun _ => liftP POST) δ h ->
-      interpret_scheap h ⊢ (⌜instprop fml ι⌝ ∧ emp) ∗ POST δ.
-    Proof.
-      intros ? ? [Hfml HP].
-      transitivity (emp ∗ interpret_scheap h)%I; auto.
-      apply bi.sep_mono'; auto.
-    Qed.
-
-    Lemma assume_formula_sound {Γ Σ} {ι : Valuation Σ} {fml : Formula Σ}
-      (POST : CStore Γ -> L) :
-      forall δ h,
-        assume_formula (instprop fml ι)
-          (fun _ => liftP POST) δ h ->
-      interpret_scheap h ∗ (⌜instprop fml ι⌝ ∧ emp) ⊢ POST δ.
-    Proof.
-      iIntros (? ? HYP) "(Hh & %Hfml & _)".
-      now iApply HYP.
-    Qed.
-
-    Lemma consume_sound {Σ} {ι : Valuation Σ} {asn : Assertion Σ} (POST : L) :
-      forall h,
-      CHeapSpec.consume asn ι (fun _ h' => interpret_scheap h' ⊢ POST) h ->
-      interpret_scheap h ⊢ asn.interpret asn ι ∗ POST.
-    Proof.
-      intros ? ->%CHeapSpec.consume_sound. apply bi.sep_mono'; [easy|].
-      iIntros "(%h' & Hh' & %HΦ)". now iApply HΦ.
-    Qed.
-
-    Lemma produce_sound {Σ} {ι : Valuation Σ} {asn : Assertion Σ} (POST : L) :
-      forall h,
-        CHeapSpec.produce asn ι (fun _ h' => interpret_scheap h' ⊢ POST) h ->
-        interpret_scheap h ⊢ asn.interpret asn ι -∗ POST.
-    Proof.
-      intros ? ->%CHeapSpec.produce_sound.
-      apply bi.wand_mono'; [easy|].
-      iIntros "(%h' & Hh' & %HΦ)". now iApply HΦ.
-    Qed.
-
     Lemma call_contract_sound {Δ τ} (c : SepContract Δ τ) (args : CStore Δ)
-      (h : SCHeap) (Φ : Val τ -> L) :
-      CHeapSpec.call_contract c args (fun v h' => interpret_scheap h' ⊢ Φ v) h ->
-      CTriple (interpret_scheap h) c args Φ.
+      (Φ : Val τ → SCHeap → Prop) (h1 : SCHeap) :
+      CHeapSpec.call_contract c args Φ h1 →
+      CTriple (interpret_scheap h1) c args
+        (fun v => ∃ h' : SCHeap, interpret_scheap h' ∧ ⌜Φ v h'⌝)%I.
     Proof.
-      destruct c as [Σe δe req result ens].
-      unfold CHeapSpec.call_contract.
-      unfold CHeapSpec.bind, CHeapSpec.lift_purespec.
+      destruct c as [Σe δe req result ens]. cbn.
+      cbv [CHeapSpec.call_contract CHeapSpec.bind CHeapSpec.lift_purespec
+           CHeapSpec.demonic CPureSpec.demonic].
       rewrite CPureSpec.wp_angelic_ctx.
       intros [ι Hwp]; revert Hwp.
       rewrite CPureSpec.wp_assert_eq_nenv.
-      intros [Hfmls Hwp]. cbn.
+      intros [Hfmls ->%CHeapSpec.consume_sound].
       apply bi.exist_intro' with ι.
       apply bi.and_intro; auto.
-      apply consume_sound.
-      revert Hwp.
-      apply CHeapSpec.mon_consume.
-      intros _ _ _ h' Hwp. hnf in Hwp.
-      apply bi.forall_intro; intro v.
-      specialize (Hwp v).
-      now apply produce_sound.
+      apply bi.sep_mono'; auto.
+      apply bi.exist_elim. intros h'.
+      apply bi.pure_elim_r.
+      intros Hwp. apply bi.forall_intro; intro v.
+      specialize (Hwp v). now apply CHeapSpec.produce_sound in Hwp.
     Qed.
 
     Lemma call_lemma_sound [Δ] (l : Lemma Δ) (δ : CStore Δ)
@@ -292,12 +111,16 @@ Module Type Soundness
       apply CHeapSpec.produce_sound.
     Qed.
 
-    Definition SoundExec (rec : Exec) :=
+    Definition SoundExec (exec : Exec) :=
       forall
-        Γ σ (s : Stm Γ σ) (POST : Val σ -> CStore Γ -> L)
+        Γ σ (s : Stm Γ σ) (Φ : Val σ → CStore Γ → SCHeap → Prop)
         (δ1 : CStore Γ) (h1 : SCHeap),
-        rec _ _ s (fun v => liftP (POST v)) δ1 h1 ->
-        ⦃ interpret_scheap h1 ⦄ s ; δ1 ⦃ POST ⦄.
+        exec _ _ s Φ δ1 h1 ->
+        ⦃ interpret_scheap h1 ⦄
+          s ; δ1
+        ⦃ fun v δ' =>
+            ∃ h' : SCHeap, interpret_scheap h' ∧ ⌜Φ v δ' h'⌝
+        ⦄.
 
     Lemma exec_aux_sound rec (rec_mono : MonotonicExec rec) (rec_sound : SoundExec rec) :
       SoundExec (exec_aux rec).
@@ -310,28 +133,28 @@ Module Type Soundness
         cbn; intros HYP.
 
       - (* stm_val *)
-        now apply rule_stm_val.
+        apply rule_stm_val.
+        apply bi.exist_intro' with h1.
+        apply bi.and_intro.
+        reflexivity.
+        apply bi.pure_intro.
+        auto.
 
       - (* stm_exp *)
-        now apply rule_stm_exp.
+        apply rule_stm_exp.
+        apply bi.exist_intro' with h1.
+        apply bi.and_intro.
+        reflexivity.
+        apply bi.pure_intro.
+        auto.
 
       - (* stm_let *)
-        eapply rule_consequence_left.
-        eapply rule_stm_let; intros; apply rule_wp.
-
-        apply bi.exist_intro' with (interpret_scheap h1).
-        apply bi.and_intro.
-        reflexivity.
-        apply bi.pure_intro.
-        apply IHs1; clear IHs1.
-        revert HYP. apply exec_aux_monotonic; auto.
-        intros v2 δ2 h2. intros HYP.
-        apply bi.exist_intro' with (interpret_scheap h2).
-        apply bi.and_intro.
-        reflexivity.
-        apply bi.pure_intro.
-        apply IHs2.
-        auto.
+        eapply rule_stm_let.
+        apply IHs1, HYP. clear IHs1 HYP.
+        intros v1 δ2.
+        apply rule_exist. intros h.
+        apply rule_pull. intros HYP.
+        now apply IHs2.
 
       - (* stm_block *)
         now apply rule_stm_block, IHs.
@@ -355,22 +178,18 @@ Module Type Soundness
 
       - (* stm_lemmak *)
         eapply rule_stm_lemmak.
-        apply (call_lemma_sound _ _ _ _ HYP).
+        apply (call_lemma_sound _ _ _ _ HYP). clear HYP.
         apply rule_exist. intros h.
-        apply rule_pull.
+        apply rule_pull. intros HYP.
         now apply IHs.
 
       - (* stm_seq *)
-        apply rule_stm_seq with (fun _ => WP s2 POST).
-        + apply IHs1. revert HYP.
-          apply exec_aux_monotonic; auto.
-          intros _ δ1' h1' H.
-          specialize (IHs2 POST δ1' h1' H).
-          unfold liftP, WP.
-          apply bi.exist_intro' with (interpret_scheap h1').
-          apply bi.and_intro. reflexivity.
-          apply bi.pure_intro. assumption.
-        + intros. apply rule_wp.
+        eapply rule_stm_seq.
+        apply IHs1, HYP. clear IHs1 HYP.
+        intros v1 δ2.
+        apply rule_exist. intros h.
+        apply rule_pull. intros HYP.
+        now apply IHs2.
 
       - (* stm_assert *)
         apply rule_stm_assert; intro Heval.
@@ -382,34 +201,14 @@ Module Type Soundness
         apply bi.True_intro.
 
       - (* stm_match_newpattern *)
-        apply
-          (rule_consequence_left
-             (WP s
-                (fun (vσ : Val σ) (δ2 : CStore Γ) =>
-                   let 'existT pc δpc := pattern_match_val pat vσ in
-                   WP (rhs pc)
-                     (fun vτ δ3  => POST vτ (env.drop (PatternCaseCtx pc) δ3))
-                     (δ2 ►► δpc))
-                δ1)).
-        + eapply rule_stm_pattern_match.
-          apply rule_wp. intros.
-          eapply rule_consequence_left.
-          apply rule_wp.
-          now rewrite pattern_match_val_inverse_right.
-        + apply bi.exist_intro' with (interpret_scheap h1).
-          apply bi.and_intro.
-          reflexivity.
-          apply bi.pure_intro.
-          apply IHs; clear IHs.
-          revert HYP. apply exec_aux_monotonic; auto.
-          intros v2 δ2 h2 HYP; cbn.
-          rewrite wp_demonic_pattern_match in HYP.
-          destruct pattern_match_val. cbn in HYP.
-          apply bi.exist_intro' with (interpret_scheap h2).
-          apply bi.and_intro.
-          reflexivity.
-          apply bi.pure_intro.
-          now apply H.
+        eapply rule_stm_pattern_match.
+        apply IHs, HYP. clear IHs HYP.
+        intros pc δpc δΓ'. cbn.
+        apply rule_exist. intros h.
+        apply rule_pull. intros HYP.
+        apply wp_demonic_pattern_match in HYP.
+        rewrite pattern_match_val_inverse_right in HYP.
+        now apply H.
 
       - (* stm_read_register *)
         destruct HYP as [v HYP].
@@ -420,10 +219,7 @@ Module Type Soundness
         apply bi.sep_mono'. easy.
         apply bi.exist_elim. intros h2.
         apply bi.pure_elim_r.
-        intros ->%CPureSpec.wp_produce_chunk.
-        apply bi.wand_mono'. easy.
-        apply bi.exist_elim. intros h3.
-        now apply bi.pure_elim_r.
+        now intros ->%CPureSpec.wp_produce_chunk.
 
       - (* stm_write_register *)
         destruct HYP as [v HYP].
@@ -434,73 +230,25 @@ Module Type Soundness
         apply bi.sep_mono'. easy.
         apply bi.exist_elim. intros h2.
         apply bi.pure_elim_r.
-        intros ->%CPureSpec.wp_produce_chunk.
-        apply bi.wand_mono'. easy.
-        apply bi.exist_elim. intros h3.
-        now apply bi.pure_elim_r.
+        now intros ->%CPureSpec.wp_produce_chunk.
 
       - (* stm_bind *)
-        eapply rule_consequence_left.
-        eapply rule_stm_bind; intros; apply rule_wp.
-
-        apply bi.exist_intro' with (interpret_scheap h1).
-        apply bi.and_intro.
-        reflexivity.
-        apply bi.pure_intro.
-        apply IHs; clear IHs.
-        revert HYP. apply exec_aux_monotonic; auto.
-        intros v2 δ2 h2 HYP; cbn.
-
-        apply bi.exist_intro' with (interpret_scheap h2).
-        apply bi.and_intro.
-        reflexivity.
-        apply bi.pure_intro.
+        eapply rule_stm_bind.
+        apply IHs, HYP. clear IHs HYP.
+        intros v1 δ2. cbn.
+        apply rule_exist. intros h.
+        apply rule_pull. intros HYP.
         now apply H.
-      - constructor. auto.
+
+      - (* stm_debug *)
+        constructor. auto.
     Qed.
 
     Lemma exec_sound n : SoundExec (@exec n).
     Proof.
       induction n; cbn.
       - unfold SoundExec; cbn; contradiction.
-      - apply exec_aux_sound; auto using exec_monotonic.
-    Qed.
-
-    Lemma exec_sound_forwards {n Γ σ} (s : Stm Γ σ) Φ δ1 h1 :
-      exec n s Φ δ1 h1 ->
-      ⦃ interpret_scheap h1 ⦄ s; δ1
-      ⦃ fun v δ2 => ∃ h, interpret_scheap h ∧ ⌜Φ v δ2 h⌝ ⦄.
-    Proof.
-      intros HΦ. apply (exec_sound n). revert HΦ. apply exec_monotonic.
-      unfold liftP. intros v δ h HΦ. apply bi.exist_intro' with h. auto.
-    Qed.
-
-    Lemma exec_sound' n {Γ σ} (s : Stm Γ σ) (POST : Val σ -> CStore Γ -> L) :
-      forall δ1 h1,
-        exec n s (fun v2 => liftP (POST v2)) δ1 h1 ->
-        liftP (WP s POST) δ1 h1.
-    Proof.
-      cbn in *; intros.
-      unfold WP.
-      apply exec_sound in H.
-      apply bi.exist_intro' with (interpret_scheap h1).
-      apply bi.and_intro.
-      reflexivity.
-      now apply bi.pure_intro.
-    Qed.
-
-    Lemma exec_sound_forwards' {n Γ σ} (s : Stm Γ σ) Φ δ1 h1 :
-      exec n s Φ δ1 h1 ->
-      interpret_scheap h1 ⊢
-      WP s (fun v δ2 => ∃ h2, interpret_scheap h2 ∧ ⌜Φ v δ2 h2⌝) δ1.
-    Proof.
-      cbn in *; intros.
-      unfold WP.
-      apply exec_sound_forwards in H.
-      apply bi.exist_intro' with (interpret_scheap h1).
-      apply bi.and_intro.
-      reflexivity.
-      now apply bi.pure_intro.
+      - apply exec_aux_sound; auto using mon_exec.
     Qed.
 
     Lemma vcgen_sound n {Δ τ} (c : SepContract Δ τ) (body : Stm Δ τ) :
@@ -516,15 +264,10 @@ Module Type Soundness
       specialize (HYP ι). remember (inst δΣ ι) as δ.
       apply CHeapSpec.produce_sound, wand_sep_adjoint in HYP. cbn in HYP.
       rewrite bi.emp_sep in HYP.
-      eapply rule_consequence_left.
-      apply rule_wp. rewrite HYP. clear HYP.
-      apply bi.exist_elim. intros h1.
-      apply bi.pure_elim_r. intros HΦ%exec_sound_forwards'.
-      rewrite HΦ. clear HΦ. unfold WP.
-      apply bi.exist_mono; intros P.
-      apply bi.and_mono; auto.
-      apply bi.pure_mono. intros Htriple.
-      apply (rule_consequence_right _ Htriple). clear Htriple. intros.
+      refine (rule_consequence_left _ _ HYP). clear HYP.
+      apply rule_exist. intros h1.
+      apply rule_pull. intros HΦ%exec_sound.
+      apply (rule_consequence_right _ HΦ). clear HΦ. intros.
       apply bi.exist_elim. intros h2.
       apply bi.pure_elim_r. intros Hheap%CHeapSpec.consume_sound.
       rewrite Hheap.
